src/ssa/opsem_inst.v
@@ -1,0 +1,1585 @@
+Add LoadPath "./ott".
+Add LoadPath "./monads".
+Add LoadPath "./compcert".
+Add LoadPath "../../../theory/metatheory_8.3".
+Require Import Ensembles.
+Require Import ssa_def.
+Require Import ssa_lib.
+Require Import ssa_props.
+Require Import ssa_analysis.
+Require Import ssa_static.
+Require Import ssa_static_lib.
+Require Import List.
+Require Import Arith.
+Require Import tactics.
+Require Import monad.
+Require Import trace.
+Require Import Metatheory.
+Require Import genericvalues.
+Require Import alist.
+Require Import Values.
+Require Import Memory.
+Require Import Integers.
+Require Import Coqlib.
+Require Import targetdata.
+Require Import Floats.
+Require Import AST.
+Require Import Maps.
+Require Import opsem.
+
+Module OpsemProps (GVsSig : GenericValuesSig).
+
+Module OS := Opsem GVsSig.
+Export OS.
+
+Lemma BOP_inversion : forall TD lc gl b s v1 v2 gv2,
+  BOP TD lc gl b s v1 v2 = Some gv2 ->
+  exists gvs1, exists gvs2,
+    getOperandValue TD v1 lc gl = Some gvs1 /\
+    getOperandValue TD v2 lc gl = Some gvs2 /\
+    GVsSig.lift_op2 (mbop TD b s) gvs1 gvs2 (typ_int s) = gv2.
+Proof.
+  intros TD lc gl b s v1 v2 gv2 HBOP.
+  unfold BOP in HBOP.
+  remember (getOperandValue TD v1 lc gl) as ogv1.
+  destruct ogv1; try solve [inversion HBOP]. 
+  remember (getOperandValue TD v2 lc gl) as ogv2.
+  destruct ogv2; inv HBOP.
+  eauto.
+Qed.
+
+Lemma FBOP_inversion : forall TD lc gl b fp v1 v2 gv,
+  FBOP TD lc gl b fp v1 v2 = Some gv ->
+  exists gv1, exists gv2,
+    getOperandValue TD v1 lc gl = Some gv1 /\
+    getOperandValue TD v2 lc gl = Some gv2 /\
+    GVsSig.lift_op2 (mfbop TD b fp) gv1 gv2 (typ_floatpoint fp) = gv.
+Proof.
+  intros TD lc gl b fp v1 v2 gv HFBOP.
+  unfold FBOP in HFBOP.
+  remember (getOperandValue TD v1 lc gl) as ogv1.
+  destruct ogv1; try solve [inversion HFBOP].
+  remember (getOperandValue TD v2 lc gl) as ogv2.
+  destruct ogv2; inv HFBOP.
+  eauto.
+Qed.
+
+Lemma CAST_inversion : forall TD lc gl op t1 v1 t2 gv,
+  CAST TD lc gl op t1 v1 t2 = Some gv ->
+  exists gv1,
+    getOperandValue TD v1 lc gl = Some gv1 /\
+    GVsSig.lift_op1 (mcast TD op t1 t2) gv1 t2 = gv.
+Proof.
+  intros TD lc gl op t1 v1 t2 gv HCAST.
+  unfold CAST in HCAST.
+  remember (getOperandValue TD v1 lc gl) as ogv1.
+  destruct ogv1; inv HCAST.
+  eauto.
+Qed.
+
+Lemma TRUNC_inversion : forall TD lc gl op t1 v1 t2 gv,
+  TRUNC TD lc gl op t1 v1 t2 = Some gv ->
+  exists gv1,
+    getOperandValue TD v1 lc gl = Some gv1 /\
+    GVsSig.lift_op1 (mtrunc TD op t1 t2) gv1 t2 = gv.
+Proof.
+  intros TD lc gl op t1 v1 t2 gv HTRUNC.
+  unfold TRUNC in HTRUNC.
+  remember (getOperandValue TD v1 lc gl) as ogv1.
+  destruct ogv1; inv HTRUNC.
+  eauto.
+Qed.
+
+Lemma EXT_inversion : forall TD lc gl op t1 v1 t2 gv,
+  EXT TD lc gl op t1 v1 t2 = Some gv ->
+  exists gv1,
+    getOperandValue TD v1 lc gl = Some gv1 /\
+    GVsSig.lift_op1 (mext TD op t1 t2) gv1 t2 = gv.
+Proof.
+  intros TD lc gl op t1 v1 t2 gv HEXT.
+  unfold EXT in HEXT.
+  remember (getOperandValue TD v1 lc gl) as ogv1.
+  destruct ogv1; inv HEXT.
+  eauto.
+Qed.
+
+Lemma ICMP_inversion : forall TD lc gl cond t v1 v2 gv,
+  ICMP TD lc gl cond t v1 v2 = Some gv ->
+  exists gv1, exists gv2,
+    getOperandValue TD v1 lc gl = Some gv1 /\
+    getOperandValue TD v2 lc gl = Some gv2 /\
+    GVsSig.lift_op2 (micmp TD cond t) gv1 gv2 (typ_int 1%nat) = gv.
+Proof.
+  intros TD lc gl cond0 t v1 v2 gv HICMP.
+  unfold ICMP in HICMP.
+  remember (getOperandValue TD v1 lc gl) as ogv1.
+  destruct ogv1; try solve [inversion HICMP].
+  remember (getOperandValue TD v2 lc gl) as ogv2.
+  destruct ogv2; inv HICMP.
+  eauto.
+Qed.
+
+Lemma FCMP_inversion : forall TD lc gl cond fp v1 v2 gv,
+  FCMP TD lc gl cond fp v1 v2 = Some gv ->
+  exists gv1, exists gv2,
+    getOperandValue TD v1 lc gl = Some gv1 /\
+    getOperandValue TD v2 lc gl = Some gv2 /\
+    GVsSig.lift_op2 (mfcmp TD cond fp) gv1 gv2 (typ_int 1%nat) = gv.
+Proof.
+  intros TD lc gl cond0 fp v1 v2 gv HFCMP.
+  unfold FCMP in HFCMP.
+  remember (getOperandValue TD v1 lc gl) as ogv1.
+  destruct ogv1; try solve [inversion HFCMP].
+  remember (getOperandValue TD v2 lc gl) as ogv2.
+  destruct ogv2; inv HFCMP.
+  eauto.
+Qed.
+
+(*
+Lemma GEP_inversion : forall (TD:TargetData) (t:typ) (ma:GenericValue) 
+  (vidxs:list GenericValue) ib mptr0,
+  GEP TD t ma vidxs ib = Some mptr0 ->
+  exists idxs, exists ptr, exists ptr0, 
+    GVs2Nats TD vidxs = Some idxs /\ 
+    GV2ptr TD (getPointerSize TD) ma = Some ptr /\
+    mgep TD t ptr idxs = Some ptr0 /\
+    ptr2GV TD ptr0 = mptr0.
+Proof.
+  intros.
+  unfold GEP in H.
+  remember (GVs2Nats TD vidxs) as oidxs.
+  remember (GV2ptr TD (getPointerSize TD) ma) as R.
+  destruct R.
+    destruct oidxs.
+      remember (mgep TD t v l0) as og.
+      destruct og; inversion H; subst.
+        exists l0. exists v. exists v0. auto.
+        exists l0. exists v. exists v0. auto.
+
+Qed.
+*)
+
+Lemma const2GV_eqAL : forall c gl1 gl2 TD, 
+  eqAL _ gl1 gl2 -> 
+  const2GV TD gl1 c = const2GV TD gl2 c.
+Proof.
+  intros. unfold const2GV.
+  destruct const2GV_eqAL_aux.
+  erewrite H0; eauto.
+Qed.
+
+Lemma getOperandValue_eqAL : forall lc1 gl lc2 v TD,
+  eqAL _ lc1 lc2 ->
+  getOperandValue TD v lc1 gl = getOperandValue TD v lc2 gl.
+Proof.
+  intros lc1 gl lc2 v TD HeqAL.
+  unfold getOperandValue in *.
+  destruct v; auto.
+Qed.
+
+Lemma BOP_eqAL : forall lc1 gl lc2 bop0 sz0 v1 v2 TD,
+  eqAL _ lc1 lc2 ->
+  BOP TD lc1 gl bop0 sz0 v1 v2 = BOP TD lc2 gl bop0 sz0 v1 v2.
+Proof.
+  intros lc1 gl lc2 bop0 sz0 v1 v2 TD HeqEnv.
+  unfold BOP in *.
+  rewrite getOperandValue_eqAL with (lc2:=lc2)(v:=v1); auto.
+  rewrite getOperandValue_eqAL with (lc2:=lc2)(v:=v2); auto.
+Qed.
+
+Lemma FBOP_eqAL : forall lc1 gl lc2 fbop0 fp0 v1 v2 TD,
+  eqAL _ lc1 lc2 ->
+  FBOP TD lc1 gl fbop0 fp0 v1 v2 = FBOP TD lc2 gl fbop0 fp0 v1 v2.
+Proof.
+  intros lc1 gl lc2 fbop0 fp0 v1 v2 TD HeqEnv.
+  unfold FBOP in *.
+  rewrite getOperandValue_eqAL with (lc2:=lc2)(v:=v1); auto.
+  rewrite getOperandValue_eqAL with (lc2:=lc2)(v:=v2); auto.
+Qed.
+
+Lemma CAST_eqAL : forall lc1 gl lc2 op t1 v1 t2 TD,
+  eqAL _ lc1 lc2 ->
+  CAST TD lc1 gl op t1 v1 t2 = CAST TD lc2 gl op t1 v1 t2.
+Proof.
+  intros lc1 gl lc2 op t1 v1 t2 TD HeqAL.
+  unfold CAST in *.
+  rewrite getOperandValue_eqAL with (lc2:=lc2)(v:=v1); auto.
+Qed.
+
+Lemma TRUNC_eqAL : forall lc1 gl lc2 op t1 v1 t2 TD,
+  eqAL _ lc1 lc2 ->
+  TRUNC TD lc1 gl op t1 v1 t2 = TRUNC TD lc2 gl op t1 v1 t2.
+Proof.
+  intros lc1 gl lc2 op t1 v1 t2 TD HeqAL.
+  unfold TRUNC in *.
+  rewrite getOperandValue_eqAL with (lc2:=lc2)(v:=v1); auto.
+Qed.
+
+Lemma EXT_eqAL : forall lc1 gl lc2 op t1 v1 t2 TD,
+  eqAL _ lc1 lc2 ->
+  EXT TD lc1 gl op t1 v1 t2 = EXT TD lc2 gl op t1 v1 t2.
+Proof.
+  intros lc1 gl lc2 op t1 v1 t2 TD HeqAL.
+  unfold EXT in *.
+  rewrite getOperandValue_eqAL with (lc2:=lc2)(v:=v1); auto.
+Qed.
+
+Lemma ICMP_eqAL : forall lc1 gl lc2 cond t v1 v2 TD,
+  eqAL _ lc1 lc2 ->
+  ICMP TD lc1 gl cond t v1 v2 = ICMP TD lc2 gl cond t v1 v2.
+Proof.
+  intros lc1 gl lc2 cond0 t v1 v2 TD HeqAL.
+  unfold ICMP in *.
+  rewrite getOperandValue_eqAL with (lc2:=lc2)(v:=v1); auto.
+  rewrite getOperandValue_eqAL with (lc2:=lc2)(v:=v2); auto.
+Qed.
+
+Lemma FCMP_eqAL : forall lc1 gl lc2 cond fp v1 v2 TD,
+  eqAL _ lc1 lc2 ->
+  FCMP TD lc1 gl cond fp v1 v2 = FCMP TD lc2 gl cond fp v1 v2.
+Proof.
+  intros lc1 gl lc2 cond0 fp v1 v2 TD HeqAL.
+  unfold FCMP in *.
+  rewrite getOperandValue_eqAL with (lc2:=lc2)(v:=v1); auto.
+  rewrite getOperandValue_eqAL with (lc2:=lc2)(v:=v2); auto.
+Qed.
+
+Lemma values2GVs_eqAL : forall l0 lc1 gl lc2 TD,
+  eqAL _ lc1 lc2 ->
+  values2GVs TD l0 lc1 gl = values2GVs TD l0 lc2 gl.
+Proof.
+  induction l0; intros lc1 gl lc2 TD HeqAL; simpl; auto.
+    rewrite getOperandValue_eqAL with (lc2:=lc2)(v:=v); auto.
+    erewrite IHl0; eauto.
+Qed.
+(*
+Lemma lookupFdefViaGV_inversion : forall TD Ps gl lc fs fv f,
+  lookupFdefViaGV TD Ps gl lc fs fv = Some f ->
+  exists fptr, exists fn,
+    getOperandValue TD fv lc gl = Some fptr /\
+    lookupFdefViaGVFromFunTable fs fptr = Some fn /\
+    lookupFdefViaIDFromProducts Ps fn = Some f.
+Proof.
+  intros.
+  unfold lookupFdefViaGV in H.
+  destruct (getOperandValue TD fv lc gl); tinv H.
+  simpl in H. exists g.
+  destruct (lookupFdefViaGVFromFunTable fs g); tinv H.
+  simpl in H. exists i0. eauto.
+Qed.  
+*)
+
+End OpsemProps.
+
+(************** Instantiate GVs ******************)
+
+Module NDGVs <: GenericValuesSig.
+
+Export LLVMsyntax.
+Export LLVMgv.
+
+Lemma singleton_inhabited : forall U (x:U), Inhabited U (Singleton U x).
+Proof.
+  intros. apply Inhabited_intro with (x:=x); auto using In_singleton.
+Qed.
+
+Lemma full_set_inhabited : forall U, 
+  (exists x:U, True) -> Inhabited U (Full_set U).
+Proof.
+  intros. inversion H.
+  apply Inhabited_intro with (x:=x); auto using Full_intro.
+Qed.
+
+Definition t := Ensemble GenericValue.
+Definition Map := list (id * t).
+Definition instantiate_gvs (gv : GenericValue) (gvs : t) : Prop :=
+  Ensembles.In _ gvs gv.
+Definition inhabited (gvs : t) : Prop := Ensembles.Inhabited _ gvs.
+Hint Unfold instantiate_gvs inhabited.
+Definition cundef_gvs gv ty : t :=
+match ty with
+| typ_int sz => fun gv => exists z, gv = (Vint sz z, Mint (sz - 1))::nil
+| typ_floatpoint fp_float => fun gv => exists f, gv = (Vfloat f, Mfloat32)::nil
+| typ_floatpoint fp_double => fun gv => exists f, gv = (Vfloat f, Mfloat64)::nil
+| typ_pointer _ => 
+    fun gv => exists b, exists ofs, gv = (Vptr b ofs, AST.Mint 31)::nil
+| _ => Singleton GenericValue gv
+end.
+
+Definition undef_gvs gv ty : t :=
+match ty with
+| typ_int sz =>
+    Ensembles.Union _ (Singleton _ gv)
+      (fun gv => exists z, gv = (Vint sz z, Mint (sz-1))::nil)
+| typ_floatpoint fp_float => 
+    Ensembles.Union _ (Singleton _ gv)
+      (fun gv => exists f, gv = (Vfloat f, Mfloat32)::nil)
+| typ_floatpoint fp_double => 
+    Ensembles.Union _ (Singleton _ gv)
+      (fun gv => exists f, gv = (Vfloat f, Mfloat64)::nil)
+| typ_pointer _ =>
+    Ensembles.Union _ (Singleton _ gv)
+      (fun gv => exists b, exists ofs, gv = (Vptr b ofs, AST.Mint 31)::nil)
+| _ => Singleton GenericValue gv
+end.
+
+Definition cgv2gvs (gv:GenericValue) ty : t :=
+match gv with
+| (Vundef, _)::nil => cundef_gvs gv ty
+| _ => Singleton _ gv
+end.
+
+Definition gv2gvs (gv:GenericValue) (ty:typ) : t :=
+match gv with
+| (Vundef, _)::nil => undef_gvs gv ty
+| _ => Singleton GenericValue gv
+end.
+
+Notation "gv @ gvs" :=  
+  (instantiate_gvs gv gvs) (at level 43, right associativity).
+Notation "$ gv # t $" := (gv2gvs gv t) (at level 41).
+
+Lemma cundef_gvs__getTypeSizeInBits : forall S los nts gv t sz al gv',
+  wf_typ S t ->
+  _getTypeSizeInBits_and_Alignment los 
+    (getTypeSizeInBits_and_Alignment_for_namedts (los,nts) true) true t = 
+      Some (sz, al) ->
+  Coqlib.nat_of_Z (Coqlib.ZRdiv (Z_of_nat sz) 8) = sizeGenericValue gv ->
+  gv' @ (cundef_gvs gv t) ->
+  Coqlib.nat_of_Z (Coqlib.ZRdiv (Z_of_nat sz) 8) = 
+    sizeGenericValue gv'.
+Proof.
+  intros S los nts gv t sz al gv' Hwft Heq1 Heq2 Hin.
+  destruct t; simpl in *;
+    try solve [inv Heq1; inv Hin; erewrite int_typsize; eauto |
+               inv Heq1; inv Hin; eauto].
+    destruct f; try solve [inv Heq1; inv Hin; eauto].
+    inv Heq1. inv Hin. inv H. simpl. auto.
+Qed.
+
+Lemma cundef_gvs__inhabited : forall gv ty, inhabited (cundef_gvs gv ty).
+Proof.
+  destruct ty; simpl; 
+    try solve [eapply Ensembles.Inhabited_intro; constructor].
+    eapply Ensembles.Inhabited_intro.
+      exists (Int.zero s). auto.
+
+    destruct f; try solve [
+      eapply Ensembles.Inhabited_intro; exists Float.zero; auto |
+      eapply Ensembles.Inhabited_intro; constructor].
+
+    eapply Ensembles.Inhabited_intro.
+      exists Mem.nullptr. exists (Int.repr 31 0). auto.
+Qed.
+
+Lemma undef_gvs__getTypeSizeInBits : forall S los nts gv t sz al gv',
+  wf_typ S t ->
+  _getTypeSizeInBits_and_Alignment los 
+    (getTypeSizeInBits_and_Alignment_for_namedts (los,nts) true) true t = 
+      Some (sz, al) ->
+  Coqlib.nat_of_Z (Coqlib.ZRdiv (Z_of_nat sz) 8) = sizeGenericValue gv ->
+  gv' @ (undef_gvs gv t) ->
+  Coqlib.nat_of_Z (Coqlib.ZRdiv (Z_of_nat sz) 8) = 
+    sizeGenericValue gv'.
+Proof.
+  intros S los nts gv t sz al gv' Hwft Heq1 Heq2 Hin.
+  destruct t; simpl in *;
+    try solve [inv Heq1; inv Hin; erewrite int_typsize; eauto |
+               inv Heq1; inv Hin; eauto].
+
+    inv Heq1; inv Hin; inv H; unfold Size.to_nat; 
+      try solve [eauto | erewrite int_typsize; eauto].
+
+    destruct f; try solve [inv Heq1; inv Hin; eauto |
+                           inv Heq1; inv Hin; inv H; auto].
+
+    inv Heq1; inv Hin; inv H; auto.
+      inv H0. auto.
+Qed.
+
+Lemma undef_gvs__inhabited : forall gv ty, inhabited (undef_gvs gv ty).
+Proof.
+  destruct ty; simpl; try solve [
+    eapply Ensembles.Inhabited_intro; apply Union_introl; constructor |
+    eapply Ensembles.Inhabited_intro; constructor].
+
+    destruct f; try solve [
+      eapply Ensembles.Inhabited_intro; apply Union_introl; constructor |
+      eapply Ensembles.Inhabited_intro; constructor].
+Qed.
+
+Lemma cgv2gvs__getTypeSizeInBits : forall S los nts gv t sz al gv',
+  wf_typ S t ->
+  _getTypeSizeInBits_and_Alignment los 
+    (getTypeSizeInBits_and_Alignment_for_namedts (los,nts) true) true t = 
+      Some (sz, al) ->
+  Coqlib.nat_of_Z (Coqlib.ZRdiv (Z_of_nat sz) 8) = sizeGenericValue gv ->
+  gv' @ (cgv2gvs gv t) ->
+  Coqlib.nat_of_Z (Coqlib.ZRdiv (Z_of_nat sz) 8) = 
+    sizeGenericValue gv'.
+Proof.
+  intros S los nts gv t sz al gv' Hwft Heq1 Heq2 Hin.
+  destruct gv; simpl in *.
+    inv Hin. simpl. auto.
+
+    destruct p.
+    destruct v; try solve [inv Hin; simpl; auto].
+    destruct gv; try solve [inv Hin; simpl; auto].
+      eapply cundef_gvs__getTypeSizeInBits in Hin; eauto.
+Qed.
+
+Lemma cgv2gvs__inhabited : forall gv t, inhabited (cgv2gvs gv t).
+Proof.
+  intros gv t.
+  destruct gv; simpl.
+    apply Ensembles.Inhabited_intro with (x:=nil).
+    apply Ensembles.In_singleton.
+
+    destruct p.
+    destruct v; auto using singleton_inhabited, cundef_gvs__inhabited.
+    destruct gv; auto using singleton_inhabited, cundef_gvs__inhabited.
+Qed.
+
+Lemma gv2gvs__getTypeSizeInBits : forall S los nts gv t sz al,
+  wf_typ S t ->
+  _getTypeSizeInBits_and_Alignment los 
+    (getTypeSizeInBits_and_Alignment_for_namedts (los,nts) true) true t = 
+      Some (sz, al) ->
+  Coqlib.nat_of_Z (Coqlib.ZRdiv (Z_of_nat sz) 8) = sizeGenericValue gv ->
+  forall gv', gv' @ (gv2gvs gv t) ->
+  sizeGenericValue gv' = Coqlib.nat_of_Z (Coqlib.ZRdiv (Z_of_nat sz) 8).
+Proof.
+  intros S los nts gv t sz al gv' Hwft Heq1 Heq2 Hin.
+  destruct gv; simpl in *.
+    inv Hin. simpl. auto.
+
+    destruct p.
+    destruct v; try solve [inv Hin; simpl; auto].
+    destruct gv; try solve [inv Hin; simpl; auto].
+      eapply undef_gvs__getTypeSizeInBits in Hin; eauto.
+Qed.
+
+Lemma gv2gvs__inhabited : forall gv t, inhabited ($ gv # t $).
+Proof.
+  intros gv t.
+  destruct gv; simpl.
+    apply Ensembles.Inhabited_intro with (x:=nil).
+    apply Ensembles.In_singleton.
+
+    destruct p.
+    destruct v; auto using singleton_inhabited, undef_gvs__inhabited.
+    destruct gv; auto using singleton_inhabited, undef_gvs__inhabited.
+Qed.
+
+Definition lift_op1 (f: GenericValue -> option GenericValue) gvs1 ty : t :=
+  fun gv2 => exists gv1, exists gv2', 
+    gv1 @ gvs1 /\ f gv1 = Some gv2' /\ (gv2 @ $ gv2' # ty $).
+
+Definition lift_op2 (f: GenericValue -> GenericValue -> option GenericValue)
+  gvs1 gvs2 ty : t :=
+  fun gv3 => exists gv1, exists gv2, exists gv3',
+    gv1 @ gvs1 /\ gv2 @ gvs2 /\ f gv1 gv2 = Some gv3' /\ (gv3 @ $ gv3' # ty $).
+
+Lemma lift_op1__inhabited : forall f gvs1 ty
+  (H:forall x, exists z, f x = Some z),
+  inhabited gvs1 -> inhabited (lift_op1 f gvs1 ty).
+Proof.
+  intros.
+  unfold lift_op1. 
+  inv H0.
+  destruct (@H x) as [z J].
+  destruct (@gv2gvs__inhabited z ty).
+  exists x0. unfold Ensembles.In. exists x. exists z.
+  rewrite J.
+  repeat (split; auto).
+Qed.
+
+Lemma lift_op2__inhabited : forall f gvs1 gvs2 ty
+  (H:forall x y, exists z, f x y = Some z),
+  inhabited gvs1 -> Ensembles.Inhabited _ gvs2 ->
+  inhabited (lift_op2 f gvs1 gvs2 ty).
+Proof.
+  intros.
+  unfold lift_op2. 
+  inv H0. inv H1.
+  destruct (@H x x0) as [z J].
+  destruct (@gv2gvs__inhabited z ty).
+  exists x1. unfold Ensembles.In. exists x. exists x0. exists z.
+  rewrite J.
+  repeat (split; auto).
+Qed.
+
+Lemma lift_op1__getTypeSizeInBits : forall S los nts f g t sz al,
+  wf_typ S t ->
+  _getTypeSizeInBits_and_Alignment los 
+    (getTypeSizeInBits_and_Alignment_for_namedts (los,nts) true) true t = 
+      Some (sz, al) ->
+  (forall x y, x @ g -> f x = Some y -> 
+   sizeGenericValue y = nat_of_Z (ZRdiv (Z_of_nat sz) 8)) ->
+  forall gv : GenericValue,
+  gv @ lift_op1 f g t ->
+  sizeGenericValue gv = nat_of_Z (ZRdiv (Z_of_nat sz) 8).
+Proof.
+  intros.
+  unfold lift_op1 in H2.
+  destruct H2 as [x [y [J1 [J2 J3]]]].
+  apply H1 in J2; auto.
+  eapply gv2gvs__getTypeSizeInBits; eauto.
+Qed.
+
+Lemma lift_op2__getTypeSizeInBits : forall S los nts f g1 g2 t sz al,
+  wf_typ S t ->
+  _getTypeSizeInBits_and_Alignment los 
+    (getTypeSizeInBits_and_Alignment_for_namedts (los,nts) true) true t = 
+      Some (sz, al) ->
+  (forall x y z, x @ g1 -> y @ g2 -> f x y = Some z -> 
+   sizeGenericValue z = nat_of_Z (ZRdiv (Z_of_nat sz) 8)) ->
+  forall gv : GenericValue,
+  gv @ lift_op2 f g1 g2 t ->
+  sizeGenericValue gv = nat_of_Z (ZRdiv (Z_of_nat sz) 8).
+Proof.
+  intros.
+  unfold lift_op2 in H2.
+  destruct H2 as [x [y [z [J1 [J2 [J3 J4]]]]]].
+  apply H1 in J3; auto.
+  eapply gv2gvs__getTypeSizeInBits; eauto.
+Qed.
+
+Lemma inhabited_inv : forall gvs, inhabited gvs -> exists gv, gv @ gvs.
+Proof.
+  intros. inv H; eauto.
+Qed.
+
+Lemma instantiate_undef__undef_gvs : forall gv t, gv @ (undef_gvs gv t).
+Proof.
+  intros. unfold undef_gvs.
+  destruct t0; try solve [apply Union_introl; constructor | constructor].
+  destruct f; try solve [apply Union_introl; constructor | constructor].
+Qed.
+
+Lemma instantiate_gv__gv2gvs : forall gv t, gv @ ($ gv # t $).
+Proof.
+  intros.
+  destruct gv; simpl; try constructor.
+  destruct p; simpl; try constructor.
+  destruct v; simpl; try constructor.
+  destruct gv; simpl; 
+    try solve [constructor | auto using instantiate_undef__undef_gvs].  
+Qed.
+
+Lemma none_undef2gvs_inv : forall gv gv' t,
+  gv @ $ gv' # t $ -> (forall mc, (Vundef, mc)::nil <> gv') -> gv = gv'.
+Proof.
+  intros.
+  destruct gv'; try solve [inv H; auto].
+  destruct p.
+  destruct v; try solve [inv H; auto].
+  destruct gv'; try solve [inv H; auto].
+  assert (J:=@H0 m). congruence.
+Qed.
+
+End NDGVs.
+
+Module DGVs <: GenericValuesSig.
+
+Export LLVMsyntax.
+Export LLVMgv.
+
+Definition t := option GenericValue.
+Definition Map := list (id * t).
+Definition instantiate_gvs (gv : GenericValue) (gvs : t) : Prop := gvs = Some gv.
+Definition inhabited (gvs : t) : Prop := gvs <> None.
+Definition cundef_gvs (gv:GenericValue) (ty:typ) : t := 
+  Some (LLVMgv.cundef_gv gv ty).
+Definition undef_gvs gv (ty:typ) : t := Some gv.
+Definition cgv2gvs (gv:GenericValue) (ty:typ) : t := Some (LLVMgv.cgv2gv gv ty).
+Definition gv2gvs (gv:GenericValue) (ty:typ) : t := Some gv.
+
+Hint Unfold instantiate_gvs inhabited.
+
+Notation "gv @ gvs" :=  
+  (instantiate_gvs gv gvs) (at level 43, right associativity).
+Notation "$ gv # t $" := (gv2gvs gv t) (at level 41).
+
+Lemma cundef_gvs__getTypeSizeInBits : forall S los nts gv ty sz al gv',
+  wf_typ S ty ->
+  _getTypeSizeInBits_and_Alignment los 
+    (getTypeSizeInBits_and_Alignment_for_namedts (los,nts) true) true ty = 
+      Some (sz, al) ->
+  Coqlib.nat_of_Z (Coqlib.ZRdiv (Z_of_nat sz) 8) = sizeGenericValue gv ->
+  gv' @ (cundef_gvs gv ty) ->
+  Coqlib.nat_of_Z (Coqlib.ZRdiv (Z_of_nat sz) 8) = 
+    sizeGenericValue gv'.
+Proof.
+  unfold instantiate_gvs. 
+  intros. inv H2.
+  eapply LLVMgv.cundef_gv__getTypeSizeInBits; eauto.
+Qed.
+
+Lemma cundef_gvs__inhabited : forall gv ty, inhabited (cundef_gvs gv ty).
+Proof. intros. unfold cundef_gvs, inhabited. congruence. Qed.
+
+Lemma undef_gvs__getTypeSizeInBits : forall S los nts gv t sz al gv',
+  wf_typ S t ->
+  _getTypeSizeInBits_and_Alignment los 
+    (getTypeSizeInBits_and_Alignment_for_namedts (los,nts) true) true t = 
+      Some (sz, al) ->
+  Coqlib.nat_of_Z (Coqlib.ZRdiv (Z_of_nat sz) 8) = sizeGenericValue gv ->
+  gv' @ (undef_gvs gv t) ->
+  Coqlib.nat_of_Z (Coqlib.ZRdiv (Z_of_nat sz) 8) = 
+    sizeGenericValue gv'.
+Proof. 
+  unfold instantiate_gvs. 
+  intros. inv H2. auto.
+Qed.
+
+Lemma undef_gvs__inhabited : forall gv ty, inhabited (undef_gvs gv ty).
+Proof. intros. unfold undef_gvs, inhabited. congruence. Qed.
+
+Lemma cgv2gvs__getTypeSizeInBits : forall S los nts gv t sz al gv',
+  wf_typ S t ->
+  _getTypeSizeInBits_and_Alignment los 
+    (getTypeSizeInBits_and_Alignment_for_namedts (los,nts) true) true t = 
+      Some (sz, al) ->
+  Coqlib.nat_of_Z (Coqlib.ZRdiv (Z_of_nat sz) 8) = sizeGenericValue gv ->
+  gv' @ (cgv2gvs gv t) ->
+  Coqlib.nat_of_Z (Coqlib.ZRdiv (Z_of_nat sz) 8) = 
+    sizeGenericValue gv'.
+Proof.
+  unfold instantiate_gvs. 
+  intros. inv H2.
+  eapply LLVMgv.cgv2gv__getTypeSizeInBits; eauto.
+Qed.
+
+Lemma cgv2gvs__inhabited : forall gv t, inhabited (cgv2gvs gv t).
+Proof. intros. unfold cgv2gvs, inhabited. congruence. Qed.
+
+Lemma gv2gvs__getTypeSizeInBits : forall S los nts gv t sz al,
+  wf_typ S t ->
+  _getTypeSizeInBits_and_Alignment los 
+    (getTypeSizeInBits_and_Alignment_for_namedts (los,nts) true) true t = 
+      Some (sz, al) ->
+  Coqlib.nat_of_Z (Coqlib.ZRdiv (Z_of_nat sz) 8) = sizeGenericValue gv ->
+  forall gv', gv' @ (gv2gvs gv t) ->
+  sizeGenericValue gv' = Coqlib.nat_of_Z (Coqlib.ZRdiv (Z_of_nat sz) 8).
+Proof.
+  unfold instantiate_gvs. 
+  intros. inv H2. auto.
+Qed.
+
+Lemma gv2gvs__inhabited : forall gv t, inhabited ($ gv # t $).
+Proof. intros. unfold gv2gvs, inhabited. congruence. Qed.
+
+Definition lift_op1 (f: GenericValue -> option GenericValue) gvs1 (ty:typ) : t :=
+match gvs1 with
+| Some gv1 => f gv1
+| _ => None
+end.
+
+Definition lift_op2 (f: GenericValue -> GenericValue -> option GenericValue)
+  gvs1 gvs2 (ty: typ) : t := 
+match gvs1, gvs2 with
+| Some gv1, Some gv2 => f gv1 gv2
+| _, _ => None
+end.
+
+Lemma lift_op1__inhabited : forall f gvs1 ty
+  (H:forall x, exists z, f x = Some z),
+  inhabited gvs1 -> inhabited (lift_op1 f gvs1 ty).
+Proof.
+  intros.
+  unfold lift_op1. 
+  destruct gvs1; eauto.
+  destruct (@H g) as [z J].
+  rewrite J. congruence.
+Qed.
+
+Lemma lift_op2__inhabited : forall f gvs1 gvs2 t
+  (H:forall x y, exists z, f x y = Some z),
+  inhabited gvs1 -> inhabited gvs2 ->
+  inhabited (lift_op2 f gvs1 gvs2 t).
+Proof.
+  intros.
+  unfold lift_op2. 
+  destruct gvs1; eauto.
+  destruct gvs2; eauto.
+  destruct (@H g g0) as [z J].
+  rewrite J. congruence.
+Qed.
+
+Lemma lift_op1__getTypeSizeInBits : forall S los nts f g t sz al,
+  wf_typ S t ->
+  _getTypeSizeInBits_and_Alignment los 
+    (getTypeSizeInBits_and_Alignment_for_namedts (los,nts) true) true t = 
+      Some (sz, al) ->
+  (forall x y, x @ g -> f x = Some y -> 
+   sizeGenericValue y = nat_of_Z (ZRdiv (Z_of_nat sz) 8)) ->
+  forall gv : GenericValue,
+  gv @ lift_op1 f g t ->
+  sizeGenericValue gv = nat_of_Z (ZRdiv (Z_of_nat sz) 8).
+Proof.
+  intros.
+  unfold lift_op1, instantiate_gvs in H2.
+  destruct g; tinv H2.
+  apply H1 in H2; auto.
+Qed.
+
+Lemma lift_op2__getTypeSizeInBits : forall S los nts f g1 g2 t sz al,
+  wf_typ S t ->
+  _getTypeSizeInBits_and_Alignment los 
+    (getTypeSizeInBits_and_Alignment_for_namedts (los,nts) true) true t = 
+      Some (sz, al) ->
+  (forall x y z, x @ g1 -> y @ g2 -> f x y = Some z -> 
+   sizeGenericValue z = nat_of_Z (ZRdiv (Z_of_nat sz) 8)) ->
+  forall gv : GenericValue,
+  gv @ lift_op2 f g1 g2 t ->
+  sizeGenericValue gv = nat_of_Z (ZRdiv (Z_of_nat sz) 8).
+Proof.
+  intros.
+  unfold lift_op2, instantiate_gvs in H2.
+  destruct g1; tinv H2.
+  destruct g2; tinv H2.
+  apply H1 in H2; auto.
+Qed.
+
+Lemma inhabited_inv : forall gvs, inhabited gvs -> exists gv, gv @ gvs.
+Proof.
+  intros. 
+  destruct gvs; eauto.
+    congruence.
+Qed.
+
+Lemma instantiate_undef__undef_gvs : forall gv t, gv @ (undef_gvs gv t).
+Proof. auto. Qed.
+
+Lemma instantiate_gv__gv2gvs : forall gv t, gv @ ($ gv # t $).
+Proof. auto. Qed.
+
+Lemma none_undef2gvs_inv : forall gv gv' t,
+  gv @ $ gv' # t $ -> (forall mc, (Vundef, mc)::nil <> gv') -> gv = gv'.
+Proof.
+  intros.
+  destruct gv'; try solve [inv H; auto].
+Qed.
+
+End DGVs.
+
+Module NDOS := Opsem NDGVs.
+
+Module DOS := Opsem DGVs.
+
+Module OpsemInstantiation.
+
+Module DOSprop1 := OpsemProps DGVs.
+
+Definition instantiate_gvs (gvs1:DGVs.t) (gvs2: NDGVs.t) : Prop :=
+forall gv1, 
+  DGVs.instantiate_gvs gv1 gvs1 -> NDGVs.instantiate_gvs gv1 gvs2.
+
+Hint Unfold instantiate_gvs.
+
+Lemma instantiate_gvs__incl : forall x y x0,
+  instantiate_gvs x y ->
+  DGVs.instantiate_gvs x0 x ->
+  NDGVs.instantiate_gvs x0 y.
+Proof. auto. Qed.
+
+Lemma instantiate_gvs__gv2gvs : forall gv t, 
+  instantiate_gvs (DGVs.gv2gvs gv t) (NDGVs.gv2gvs gv t).
+Proof. 
+  intros.
+  unfold DGVs.gv2gvs, NDGVs.gv2gvs.
+  destruct gv; try solve [intros gvs1 J; inv J; constructor].
+  destruct p.
+  destruct v; try solve [intros gvs1 J; inv J; constructor].
+  destruct gv; try solve [intros gvs1 J; inv J; constructor].
+  destruct t; simpl;
+    try solve [intros gvs1 J; inv J; 
+               (constructor || apply Union_introl; constructor)].
+  destruct f; simpl;
+    try solve [intros gvs1 J; inv J; 
+               (constructor || apply Union_introl; constructor)].
+Qed.
+
+Lemma instantiate_gvs__cgv2gvs : forall gv t, 
+  instantiate_gvs (DGVs.cgv2gvs gv t) (NDGVs.cgv2gvs gv t).
+Proof. 
+  intros.
+  unfold DGVs.cgv2gvs, NDGVs.cgv2gvs.
+  destruct gv; try solve [intros gvs1 J; inv J; constructor].
+  destruct p.
+  destruct v; try solve [intros gvs1 J; inv J; constructor].
+  destruct gv; try solve [intros gvs1 J; inv J; constructor].
+  destruct t; simpl;
+    try solve [intros gvs1 J; inv J;
+               try solve [constructor |
+               exists (Int.zero s); auto |
+               exists Mem.nullptr; exists (Int.repr 31 0); auto]].
+  destruct f; simpl;
+    try solve [intros gvs1 J; inv J;
+               try solve [constructor |
+               exists Float.zero; auto]].
+Qed.
+
+Lemma instantiate_gvs__lift_op1 : forall f xs1 xs2 t,
+  instantiate_gvs xs1 xs2 ->
+  instantiate_gvs (DGVs.lift_op1 f xs1 t) (NDGVs.lift_op1 f xs2 t).
+Proof.
+  intros.
+  unfold DGVs.lift_op1, NDGVs.lift_op1.
+  destruct xs1; intros gvs1 J; inv J.
+    exists g. exists gvs1. 
+    repeat (split; auto using NDGVs.instantiate_gv__gv2gvs).
+Qed.
+
+Lemma instantiate_gvs__lift_op2 : forall f xs1 ys1 xs2 ys2 t,
+  instantiate_gvs xs1 xs2 ->
+  instantiate_gvs ys1 ys2 ->
+  instantiate_gvs (DGVs.lift_op2 f xs1 ys1 t) (NDGVs.lift_op2 f xs2 ys2 t).
+Proof.
+  intros.
+  unfold DGVs.lift_op2, NDGVs.lift_op2.
+  destruct xs1; intros gvs1 J; inv J.
+  destruct ys1; tinv H2.
+    exists g. exists g0. exists gvs1. 
+    repeat (split; auto using NDGVs.instantiate_gv__gv2gvs).
+Qed.
+
+Fixpoint instantiate_locals (lc1 : DOS.GVsMap) (lc2 : NDOS.GVsMap) : Prop :=
+match lc1, lc2 with
+| nil, nil => True
+| (id1,gvs1)::lc1', (id2,gvs2)::lc2' => 
+    id1=id2 /\ instantiate_gvs gvs1 gvs2 /\ instantiate_locals lc1' lc2'
+| _, _ => False
+end.
+
+Definition instantiate_EC (ec1 : DOS.ExecutionContext) 
+  (ec2 : NDOS.ExecutionContext) : Prop :=
+match ec1, ec2 with
+| DOS.mkEC f1 b1 cs1 tmn1 lc1 als1, NDOS.mkEC f2 b2 cs2 tmn2 lc2 als2 =>
+    f1 = f2 /\ b1 = b2 /\ cs1 = cs2 /\ tmn1 = tmn2 /\
+    instantiate_locals lc1 lc2 /\ als1 = als2
+end.
+
+Fixpoint instantiate_ECs (ecs1 : DOS.ECStack) (ecs2 : NDOS.ECStack) : Prop :=
+match ecs1, ecs2 with
+| nil, nil => True
+| ec1::ecs1', ec2::ecs2' => instantiate_EC ec1 ec2 /\ instantiate_ECs ecs1' ecs2'
+| _, _ => False
+end.
+
+Definition instantiate_State (st1 : DOS.State) (st2 : NDOS.State) : Prop :=
+match st1, st2 with
+| DOS.mkState s1 td1 ps1 ecs1 gl1 fs1 M1,
+  NDOS.mkState s2 td2 ps2 ecs2 gl2 fs2 M2 =>
+    s1 = s2 /\ td1 = td2 /\ ps1 = ps2 /\ instantiate_ECs ecs1 ecs2 /\ gl1 = gl2
+    /\ fs1 = fs2 /\ M1 = M2
+end.
+
+Lemma instantiate_locals__lookup : forall lc1 lc2 id1 gv1,
+  instantiate_locals lc1 lc2 -> 
+  lookupAL _ lc1 id1 = Some gv1 ->
+  exists gvs2, lookupAL _ lc2 id1 = Some gvs2 /\ instantiate_gvs gv1 gvs2.
+Proof.
+  induction lc1; destruct lc2; simpl; intros id1 gv1 Hinst Hlk.  
+    inv Hlk.
+    inv Hinst.
+    destruct a. inv Hinst.     
+
+    destruct a. destruct p.
+    destruct Hinst as [J1 [J2 J3]]; subst.
+    destruct (id1 == i1); subst; eauto.
+      inv Hlk. eauto.
+Qed.
+
+Lemma same_singleton_set : forall gv,
+  Same_set GenericValue (Singleton _ gv) (Singleton _ gv).
+Proof.
+  unfold Same_set, Included. auto.
+Qed.
+
+Lemma instantiate_locals__getOperandValue : forall TD v lc1 lc2 gl gvs1,
+  instantiate_locals lc1 lc2 -> 
+  DOS.getOperandValue TD v lc1 gl = Some gvs1 ->
+  exists gvs2, NDOS.getOperandValue TD v lc2 gl = Some gvs2 /\
+    instantiate_gvs gvs1 gvs2.
+Proof.
+  intros.
+  destruct v; simpl in *.
+    eapply instantiate_locals__lookup; eauto.
+
+    unfold DOS.const2GV in H0. unfold NDOS.const2GV.
+    destruct (_const2GV TD gl c) as [[gv ?]|]; inv H0.
+    eauto using instantiate_gvs__cgv2gvs.
+Qed.
+
+Lemma instantiate_locals__updateAddAL : forall gvs3 gvs3',
+  instantiate_gvs gvs3 gvs3' ->
+  forall lc1 lc2 id0,
+  instantiate_locals lc1 lc2 -> 
+  instantiate_locals (updateAddAL _ lc1 id0 gvs3) (updateAddAL _ lc2 id0 gvs3').
+Proof.
+  induction lc1; destruct lc2; simpl; intros id0 H1; auto.
+    inv H1.  
+    destruct a. inv H1.
+    destruct a. destruct p. destruct H1 as [eq [H1 H2]]; subst.
+    destruct (id0 == i1); subst; simpl.
+      split; auto.
+      split; auto.
+Qed.   
+
+Lemma instantiate_locals__returnUpdateLocals : forall TD lc1 lc2 lc1' lc2' Result
+    gl lc1'' c,
+  instantiate_locals lc1 lc2 -> 
+  instantiate_locals lc1' lc2' -> 
+  DOS.returnUpdateLocals TD c Result lc1 lc1' gl = ret lc1'' ->
+  exists lc2'', 
+    NDOS.returnUpdateLocals TD c Result lc2 lc2' gl = ret lc2'' /\
+    instantiate_locals lc1'' lc2''. 
+Proof.
+  intros.
+  unfold DOS.returnUpdateLocals in H1.
+  remember (DOS.getOperandValue TD Result lc1 gl) as R.
+  destruct R; tinv H1.
+  symmetry in HeqR.
+  eapply instantiate_locals__getOperandValue in HeqR; eauto.
+  destruct HeqR as [gvs2 [J1 J2]].
+  unfold NDOS.returnUpdateLocals.
+  rewrite J1. 
+  destruct c; tinv H1.
+  destruct n; inv H1; eauto.
+  destruct t; inv H3.
+  exists (updateAddAL _ lc2' i0 (NDGVs.lift_op1 (fit_gv TD t) gvs2 t)).   
+  split; auto.
+    apply instantiate_locals__updateAddAL; auto.
+    apply instantiate_gvs__lift_op1; auto.
+Qed.
+
+Lemma instantiate_locals__getIncomingValuesForBlockFromPHINodes : forall TD b
+    gl lc1 lc2 (Hlc : instantiate_locals lc1 lc2) ps re1,  
+  DOS.getIncomingValuesForBlockFromPHINodes TD ps b gl lc1 = Some re1 ->
+  exists re2,
+    NDOS.getIncomingValuesForBlockFromPHINodes TD ps b gl lc2 = Some re2 /\
+    instantiate_locals re1 re2.
+Proof.
+  induction ps; simpl; intros.  
+    inv H. exists nil. simpl. auto.
+
+    destruct a.
+    destruct (getValueViaBlockFromValuels l0 b); tinv H.
+    remember (DOS.getOperandValue TD v lc1 gl) as R.
+    destruct R; tinv H.
+    symmetry in HeqR.  
+    eapply instantiate_locals__getOperandValue in HeqR; eauto.
+    destruct HeqR as [gvs2 [J1 J2]].
+    remember (DOS.getIncomingValuesForBlockFromPHINodes TD ps b gl lc1) as R1.
+    destruct R1; inv H.  
+    rewrite J1.
+    symmetry in HeqR1.
+    destruct (@IHps l1) as [re2 [J3 J4]]; auto.
+    rewrite J3.
+    exists ((i0, gvs2) :: re2). simpl. auto.
+Qed.
+
+Lemma instantiate_locals__updateValuesForNewBlock : forall lc1 lc2 re1 re2,
+  instantiate_locals lc1 lc2 ->
+  instantiate_locals re1 re2 ->
+  instantiate_locals (DOS.updateValuesForNewBlock re1 lc1)
+     (NDOS.updateValuesForNewBlock re2 lc2).
+Proof.
+  induction re1; destruct re2; simpl; intros; auto.
+    inv H0.
+    destruct a. inv H0.
+    destruct a. destruct p. destruct H0 as [eq [J1 J2]]; subst.
+    apply instantiate_locals__updateAddAL; auto.    
+Qed.
+
+Lemma instantiate_locals__switchToNewBasicBlock : forall TD lc1 lc2 gl lc1' b b',
+  instantiate_locals lc1 lc2 -> 
+  DOS.switchToNewBasicBlock TD b' b gl lc1 = Some lc1' ->
+  exists lc2', NDOS.switchToNewBasicBlock TD b' b gl lc2 = Some lc2' /\
+    instantiate_locals lc1' lc2'. 
+Proof.
+  intros.
+  unfold DOS.switchToNewBasicBlock in H0.
+  unfold NDOS.switchToNewBasicBlock.
+  remember (DOS.getIncomingValuesForBlockFromPHINodes TD 
+    (getPHINodesFromBlock b') b gl lc1) as R.
+  destruct R; inv H0.
+  symmetry in HeqR.
+  eapply instantiate_locals__getIncomingValuesForBlockFromPHINodes in HeqR; eauto.
+  destruct HeqR as [re2 [J1 J2]].
+  rewrite J1.
+  eauto using instantiate_locals__updateValuesForNewBlock.
+Qed.
+
+Lemma instantiate_locals__BOP : forall TD lc1 lc2 gl v1 v2 gvs3 bop sz,
+  instantiate_locals lc1 lc2 -> 
+  DOS.BOP TD lc1 gl bop sz v1 v2 = Some gvs3 ->
+  exists gvs3', NDOS.BOP TD lc2 gl bop sz v1 v2 = Some gvs3' /\
+    instantiate_gvs gvs3 gvs3'.
+Proof.
+  intros.
+  apply DOSprop1.BOP_inversion in H0.
+  destruct H0 as [gv1 [gv2 [J1 [J2 J3]]]]; subst.
+  eapply instantiate_locals__getOperandValue in J1; eauto.
+  destruct J1 as [gvs1 [H1 H2]].
+  eapply instantiate_locals__getOperandValue in J2; eauto.
+  destruct J2 as [gvs2 [H3 H4]].
+  unfold NDOS.BOP.
+  rewrite H1. rewrite H3.
+  eauto using instantiate_gvs__lift_op2.
+Qed.
+  
+Lemma instantiate_locals__FBOP : forall TD lc1 lc2 gl v1 v2 gv3 fbop fp,
+  instantiate_locals lc1 lc2 -> 
+  DOS.FBOP TD lc1 gl fbop fp v1 v2 = Some gv3 ->
+  exists gvs3', NDOS.FBOP TD lc2 gl fbop fp v1 v2 = Some gvs3' /\
+    instantiate_gvs gv3 gvs3'.
+Proof.
+  intros.
+  apply DOSprop1.FBOP_inversion in H0.
+  destruct H0 as [gv1 [gv2 [J1 [J2 J3]]]]; subst.
+  eapply instantiate_locals__getOperandValue in J1; eauto.
+  destruct J1 as [gvs1 [H1 H2]].
+  eapply instantiate_locals__getOperandValue in J2; eauto.
+  destruct J2 as [gvs2 [H3 H4]].
+  unfold NDOS.FBOP.
+  rewrite H1. rewrite H3.
+  eauto using instantiate_gvs__lift_op2.
+Qed.
+
+Lemma instantiate_locals__ICMP : forall TD lc1 lc2 gl v1 v2 gv3 c t,
+  instantiate_locals lc1 lc2 -> 
+  DOS.ICMP TD lc1 gl c t v1 v2 = Some gv3 ->
+  exists gvs3', NDOS.ICMP TD lc2 gl c t v1 v2 = Some gvs3' /\
+    instantiate_gvs gv3 gvs3'.
+Proof.
+  intros.
+  apply DOSprop1.ICMP_inversion in H0.
+  destruct H0 as [gv1 [gv2 [J1 [J2 J3]]]]; subst.
+  eapply instantiate_locals__getOperandValue in J1; eauto.
+  destruct J1 as [gvs1 [H1 H2]].
+  eapply instantiate_locals__getOperandValue in J2; eauto.
+  destruct J2 as [gvs2 [H3 H4]].
+  unfold NDOS.ICMP.
+  rewrite H1. rewrite H3.
+  eauto using instantiate_gvs__lift_op2.
+Qed.
+
+Lemma instantiate_locals__FCMP : forall TD lc1 lc2 gl v1 v2 gv3 c t,
+  instantiate_locals lc1 lc2 -> 
+  DOS.FCMP TD lc1 gl c t v1 v2 = Some gv3 ->
+  exists gvs3', NDOS.FCMP TD lc2 gl c t v1 v2 = Some gvs3' /\
+    instantiate_gvs gv3 gvs3'.
+Proof.
+  intros.
+  apply DOSprop1.FCMP_inversion in H0.
+  destruct H0 as [gv1 [gv2 [J1 [J2 J3]]]]; subst.
+  eapply instantiate_locals__getOperandValue in J1; eauto.
+  destruct J1 as [gvs1 [H1 H2]].
+  eapply instantiate_locals__getOperandValue in J2; eauto.
+  destruct J2 as [gvs2 [H3 H4]].
+  unfold NDOS.FCMP.
+  rewrite H1. rewrite H3.
+  eauto using instantiate_gvs__lift_op2.
+Qed.
+
+Definition instantiate_list_gvs (l1 : list DGVs.t) (l2 : list NDGVs.t) :=
+List.Forall2 instantiate_gvs l1 l2.
+
+Hint Unfold instantiate_list_gvs.
+
+Lemma instantiate_locals__values2GVs : forall TD lc1 lc2 gl idxs vidxs,
+  instantiate_locals lc1 lc2 -> 
+  DOS.values2GVs TD idxs lc1 gl = Some vidxs ->
+  exists vidxss, NDOS.values2GVs TD idxs lc2 gl = Some vidxss /\
+    instantiate_list_gvs vidxs vidxss.
+Proof.
+  induction idxs; simpl; intros.
+    inv H0. exists nil. auto.
+
+    remember (DOS.getOperandValue TD v lc1 gl) as R.
+    destruct R; tinv H0.
+    remember (DOS.values2GVs TD idxs lc1 gl) as R1.
+    destruct R1; inv H0.
+    symmetry in HeqR.
+    eapply instantiate_locals__getOperandValue in HeqR; eauto.
+    destruct HeqR as [gvs2 [H3 H4]].
+    destruct (@IHidxs l0) as [vidxss [J1 J2]]; auto.
+    rewrite H3. rewrite J1. eauto.
+Qed.
+
+Lemma in_instantiate_list_gvs : forall vidxss1 vidxss2 vidxs1
+  (Hinst1 : instantiate_list_gvs vidxss1 vidxss2)
+  (Hin1 : DOS.in_list_gvs vidxs1 vidxss1),
+  NDOS.in_list_gvs vidxs1 vidxss2.
+Proof.
+  intros.
+  generalize dependent vidxs1.
+  induction Hinst1; intros; inv Hin1; auto.
+    eapply IHHinst1 in H4; eauto using instantiate_gvs__incl.
+Qed.
+
+Lemma instantiate_locals__GEP : forall TD t mp1 mp1' vidxs1 vidxss1 vidxss2 
+    inbounds mps2,
+  instantiate_list_gvs vidxss1 vidxss2 ->
+  instantiate_gvs mp1 mps2 ->
+  DOS.in_list_gvs vidxs1 vidxss1 ->
+  DOS.GEP TD t mp1 vidxs1 inbounds = Some mp1' ->
+  exists vidxs2, exists mps2', 
+    NDOS.in_list_gvs vidxs2 vidxss2 /\
+    NDOS.GEP TD t mps2 vidxs2 inbounds = Some mps2' /\ 
+    instantiate_gvs mp1' mps2'.
+Proof.
+  intros TD t mp1 mp1' vidxs1 vidxss1 vidxss2 inbounds mps2 Hinst1 Hinst2 Hin1 
+    Hgep.
+  inv Hgep.
+  unfold NDOS.GEP.
+  exists vidxs1.  
+  exists (NDGVs.lift_op1 (NDOS.gep TD t vidxs1 inbounds) mps2
+           (typ_pointer (typ_int 1%nat))).
+  split; eauto using instantiate_gvs__lift_op1, in_instantiate_list_gvs.
+Qed.
+
+Lemma instantiate_locals__extractGenericValue : forall TD lc1 lc2 t gv2
+    cidxs gv1 gvs1,
+  instantiate_locals lc1 lc2 -> 
+  instantiate_gvs gv1 gvs1 ->
+  DOS.extractGenericValue TD t gv1 cidxs = Some gv2 ->
+  exists gvs2, NDOS.extractGenericValue TD t gvs1 cidxs = Some gvs2 
+    /\ instantiate_gvs gv2 gvs2.
+Proof.
+  intros.
+  unfold DOS.extractGenericValue in H1.
+  unfold NDOS.extractGenericValue.
+  destruct (intConsts2Nats TD cidxs); inv H1.
+  destruct (mgetoffset TD t l0) as [[]|]; inv H3.
+  eauto using instantiate_gvs__lift_op1.
+Qed.
+
+Lemma instantiate_locals__insertGenericValue : forall TD lc1 lc2 t1 t2 gv2 
+    cidxs gv1 gvs1 gvs2 gv3,
+  instantiate_locals lc1 lc2 -> 
+  instantiate_gvs gv1 gvs1 ->
+  instantiate_gvs gv2 gvs2 ->
+  DOS.insertGenericValue TD t1 gv1 cidxs t2 gv2 = Some gv3 ->
+  exists gvs3, NDOS.insertGenericValue TD t1 gvs1 cidxs t2 gvs2 = Some gvs3
+    /\ instantiate_gvs gv3 gvs3.
+Proof.
+  intros.
+  unfold DOS.insertGenericValue in H2.
+  unfold NDOS.insertGenericValue.
+  destruct (intConsts2Nats TD cidxs); inv H2.
+  destruct (mgetoffset TD t1 l0) as [[]|]; inv H4.
+  eauto using instantiate_gvs__lift_op2.
+Qed.
+
+Lemma instantiate_locals__CAST : forall TD lc1 lc2 gl t1 v1 t2 gv2 castop0,
+  instantiate_locals lc1 lc2 -> 
+  DOS.CAST TD lc1 gl castop0 t1 v1 t2 = Some gv2 ->
+  exists gvs2', NDOS.CAST TD lc2 gl castop0 t1 v1 t2 = Some gvs2' 
+    /\ instantiate_gvs gv2 gvs2'.
+Proof.
+  intros.
+  apply DOSprop1.CAST_inversion in H0.
+  destruct H0 as [gv1 [J1 J2]]; subst.
+  eapply instantiate_locals__getOperandValue in J1; eauto.
+  destruct J1 as [gvs1 [H1 H2]].
+  unfold NDOS.CAST.
+  rewrite H1.
+  eauto using instantiate_gvs__lift_op1.
+Qed.
+
+Lemma instantiate_locals__TRUNC : forall TD lc1 lc2 gl t1 v1 t2 gv2 top0,
+  instantiate_locals lc1 lc2 -> 
+  DOS.TRUNC TD lc1 gl top0 t1 v1 t2 = Some gv2 ->
+  exists gvs2', NDOS.TRUNC TD lc2 gl top0 t1 v1 t2 = Some gvs2' 
+    /\ instantiate_gvs gv2 gvs2'.
+Proof.
+  intros.
+  apply DOSprop1.TRUNC_inversion in H0.
+  destruct H0 as [gv1 [J1 J2]]; subst.
+  eapply instantiate_locals__getOperandValue in J1; eauto.
+  destruct J1 as [gvs1 [H1 H2]].
+  unfold NDOS.TRUNC.
+  rewrite H1.
+  eauto using instantiate_gvs__lift_op1.
+Qed.
+
+Lemma instantiate_locals__EXT : forall TD lc1 lc2 gl t1 v1 t2 gv2 top0,
+  instantiate_locals lc1 lc2 -> 
+  DOS.EXT TD lc1 gl top0 t1 v1 t2 = Some gv2 ->
+  exists gvs2', NDOS.EXT TD lc2 gl top0 t1 v1 t2 = Some gvs2' 
+    /\ instantiate_gvs gv2 gvs2'.
+Proof.
+  intros.
+  apply DOSprop1.EXT_inversion in H0.
+  destruct H0 as [gv1 [J1 J2]]; subst.
+  eapply instantiate_locals__getOperandValue in J1; eauto.
+  destruct J1 as [gvs1 [H1 H2]].
+  unfold NDOS.EXT.
+  rewrite H1.
+  eauto using instantiate_gvs__lift_op1.
+Qed.
+
+Lemma instantiate_locals__params2GVs : forall TD lc1 lc2 gl 
+  (Hlc:instantiate_locals lc1 lc2) lp gvs1,
+  DOS.params2GVs TD lp lc1 gl = Some gvs1 ->
+  exists gvss2, NDOS.params2GVs TD lp lc2 gl = Some gvss2 /\
+    instantiate_list_gvs gvs1 gvss2.
+Proof.
+  induction lp; simpl; intros.
+    inv H. eauto.
+
+    destruct a.
+    remember (DOS.getOperandValue TD v lc1 gl) as R1.
+    destruct R1; tinv H.
+    remember (DOS.params2GVs TD lp lc1 gl) as R2.
+    destruct R2; inv H.
+    symmetry in HeqR1.
+    eapply instantiate_locals__getOperandValue in HeqR1; eauto.
+    destruct HeqR1 as [gvs2 [H3 H4]].
+    destruct (@IHlp l0) as [gvsss2 [J1 J2]]; auto.
+    rewrite H3. rewrite J1. eauto.
+Qed.
+
+Lemma instantiate_locals__initializeFrameValues : forall TD lc1 lc2
+  (H2: instantiate_locals lc1 lc2) la gvs1 gvs2 lc1'
+  (H1 : instantiate_list_gvs gvs1 gvs2),
+  DOS._initializeFrameValues TD la gvs1 lc1 = Some lc1' ->
+  exists lc2',
+    NDOS._initializeFrameValues TD la gvs2 lc2 = Some lc2' /\
+    instantiate_locals lc1' lc2'.
+Proof.
+  induction la; simpl; intros.
+    inv H. eauto.
+
+    destruct a. destruct p.
+    destruct gvs1; simpl.
+      destruct gvs2; inv H1.
+      remember (DOS._initializeFrameValues TD la nil lc1) as R1.
+      destruct R1; tinv H.
+      destruct (gundef TD t); inv H.
+      symmetry in HeqR1.
+      eapply IHla in HeqR1; eauto.
+        destruct HeqR1 as [lc2' [J1 J2]].
+        unfold NDOS.GVs.
+        rewrite J1.
+        eauto using instantiate_locals__updateAddAL, instantiate_gvs__gv2gvs.
+
+      simpl in H1.
+      destruct gvs2; inv H1.
+      remember (DOS._initializeFrameValues TD la gvs1 lc1) as R1.
+      destruct R1; inv H.
+      symmetry in HeqR1.
+      eapply IHla in HeqR1; eauto.
+      destruct HeqR1 as [lc2' [J1 J2]].
+      rewrite J1.
+      eauto using instantiate_locals__updateAddAL, instantiate_gvs__lift_op1.
+Qed.           
+
+Lemma instantiate_locals__initLocals : forall TD gvs1 gvss2 
+  (H : instantiate_list_gvs gvs1 gvss2) la lc1,
+  DOS.initLocals TD la gvs1 = Some lc1 ->
+  exists lc2, 
+    NDOS.initLocals TD la gvss2 = Some lc2 /\
+    instantiate_locals lc1 lc2.
+Proof.
+  unfold DOS.initLocals, NDOS.initLocals.
+  intros.
+  eapply instantiate_locals__initializeFrameValues; eauto.
+    simpl. auto.
+Qed.
+
+Lemma instantiate_list_gvs__incl : forall x y x0,
+  instantiate_list_gvs x y ->
+  DOS.in_list_gvs x0 x ->
+  NDOS.in_list_gvs x0 y.
+Proof.
+  intros.  
+  generalize dependent x0.
+  induction H; simpl; intros.
+    inv H0; auto.
+    inv H1; auto.
+      apply IHForall2 in H6. eauto using instantiate_gvs__incl.
+Qed.
+
+Lemma instantiate_locals__exCallUpdateLocals : forall TD lc1 lc2 lc1' rid oResult
+    nr ft,
+  instantiate_locals lc1 lc2 -> 
+  DOS.exCallUpdateLocals TD ft nr rid oResult lc1 = ret lc1' ->
+  exists lc2', 
+    NDOS.exCallUpdateLocals TD ft nr rid oResult lc2 = ret lc2' /\
+    instantiate_locals lc1' lc2'. 
+Proof.
+  intros.
+  unfold DOS.exCallUpdateLocals in H0.
+  unfold NDOS.exCallUpdateLocals.
+  destruct nr; inv H0; eauto.
+  destruct oResult; inv H2; eauto.
+  destruct ft; inv H1; eauto.
+  remember (fit_gv TD ft g) as R.
+  destruct R; inv H2.
+  eauto using instantiate_locals__updateAddAL, instantiate_gvs__gv2gvs.
+Qed.
+
+Tactic Notation "sInsn_cases" tactic(first) tactic(c) :=
+  first;
+  [ c "sReturn" | c "sReturnVoid" | c "sBranch" | c "sBranch_uncond" |
+    c "sBop" | c "sFBop" | c "sExtractValue" | c "sInsertValue" |
+    c "sMalloc" | c "sFree" |
+    c "sAlloca" | c "sLoad" | c "sStore" | c "sGEP" |
+    c "sTrunc" | c "sExt" | 
+    c "sCast" | 
+    c "sIcmp" | c "sFcmp" | c "sSelect" |  
+    c "sCall" | c "sExCall" ].
+
+Ltac simpl_nd_llvmds :=
+  match goal with
+  | [Hsim : instantiate_State {| DOS.ECS := _::_::_ |} ?st2 |- _ ] =>
+     destruct st2 as [S' TD' Ps' ECs' gl' fs' M'];
+     destruct Hsim as [eq1 [eq2 [eq3 [Hsim [eq4 [eq5 eq6]]]]]]; subst;
+     destruct ECs' as [|[f1' b1' cs1' tmn1' lc1' als1'] ECs']; 
+       try solve [inversion Hsim];
+     simpl in Hsim; destruct Hsim as [Hsim1 Hsim2];
+     destruct ECs' as [|[f2' b2' cs2' tmn2' lc2' als2'] ECs'];
+       try solve [inversion Hsim2];
+     destruct Hsim2 as [Hsim2 Hsim3];
+     destruct Hsim1 as [J1 [J2 [J3 [J4 [Hsim1 J6]]]]]; subst;
+     destruct Hsim2 as [J1 [J2 [J3 [J4 [Hsim2 J6]]]]]; subst
+  | [Hsim : instantiate_State {| DOS.ECS := _::_|} ?st2 |- _ ] =>
+     destruct st2 as [S' TD' Ps' ECs' gl' fs' M'];
+     destruct Hsim as [eq1 [eq2 [eq3 [Hsim [eq4 [eq5 eq6]]]]]]; subst;
+     destruct ECs' as [|[f1' b1' cs1' tmn1' lc1' als1'] ECs']; 
+       try solve [inversion Hsim];
+     simpl in Hsim; destruct Hsim as [Hsim1 Hsim2];
+     destruct Hsim1 as [J1 [J2 [J3 [J4 [Hsim1 J6]]]]]; subst
+  end.
+
+Lemma instantiate_dsInsn : forall st1 st2 st1' tr,
+  instantiate_State st1 st2 ->
+  DOS.sInsn st1 st1' tr ->
+  (exists st2', NDOS.sInsn st2 st2' tr /\ instantiate_State st1' st2').
+Proof.
+  intros st1 st2 st1' tr Hsim Hop.  
+  (sInsn_cases (induction Hop) Case).
+Case "sReturn". simpl_nd_llvmds. 
+  eapply instantiate_locals__returnUpdateLocals in H1; eauto.
+  destruct H1 as [lc2'' [H1 H2]].
+  exists (NDOS.mkState S' TD' Ps' 
+    ((NDOS.mkEC f2' b2' cs' tmn2' lc2'' als2')::ECs') gl' fs' Mem').
+  split; eauto.
+    repeat (split; auto).
+Case "sReturnVoid". simpl_nd_llvmds. 
+  exists (NDOS.mkState S' TD' Ps' 
+    ((NDOS.mkEC f2' b2' cs' tmn2' lc2' als2')::ECs') gl' fs' Mem').
+  split; eauto.
+    repeat (split; auto).
+Case "sBranch". simpl_nd_llvmds. 
+  eapply instantiate_locals__switchToNewBasicBlock in H2; eauto.
+  eapply instantiate_locals__getOperandValue in H; eauto.
+  destruct H as [gvs2 [J1 J2]].
+  destruct H2 as [lc2' [J3 J4]].
+  exists (NDOS.mkState S' TD' Ps' 
+    ((NDOS.mkEC f1' (block_intro l' ps' cs' tmn') cs' tmn' lc2' als1')
+      ::ECs') gl' fs' M').
+  split; eauto using instantiate_gvs__incl.
+    repeat (split; auto).
+Case "sBranch_uncond". simpl_nd_llvmds. 
+  eapply instantiate_locals__switchToNewBasicBlock in H0; eauto.
+  destruct H0 as [lc2' [J1 J2]]. 
+  exists (NDOS.mkState S' TD' Ps' 
+    ((NDOS.mkEC f1' (block_intro l' ps' cs' tmn') cs' tmn' lc2' als1')
+      ::ECs') gl' fs' M').
+  split; eauto.
+    repeat (split; auto).
+Case "sBop". simpl_nd_llvmds. 
+  eapply instantiate_locals__BOP in H; eauto.
+  destruct H as [gvs3' [J1 J2]].
+  exists (NDOS.mkState S' TD' Ps' 
+    ((NDOS.mkEC f1' b1' cs tmn1' (updateAddAL _ lc1' id0 gvs3') als1')
+      ::ECs') gl' fs' M').
+  split; eauto.
+    repeat (split; auto using instantiate_locals__updateAddAL).
+Case "sFBop". simpl_nd_llvmds. 
+  eapply instantiate_locals__FBOP in H; eauto.
+  destruct H as [gvs3' [J1 J2]]. 
+  exists (NDOS.mkState S' TD' Ps' 
+    ((NDOS.mkEC f1' b1' cs tmn1' (updateAddAL _ lc1' id0 gvs3') als1')
+      ::ECs') gl' fs' M').
+  split; eauto.
+    repeat (split; auto using instantiate_locals__updateAddAL).
+Case "sExtractValue". simpl_nd_llvmds. 
+  eapply instantiate_locals__getOperandValue in H; eauto.
+  destruct H as [gvs2 [J1 J2]].
+  eapply instantiate_locals__extractGenericValue in H0; eauto.
+  destruct H0 as [gvs2' [J3 J4]].
+  exists (NDOS.mkState S' TD' Ps' 
+    ((NDOS.mkEC f1' b1' cs tmn1' (updateAddAL _ lc1' id0 gvs2') als1')
+      ::ECs') gl' fs' M').
+  split; eauto.
+    repeat (split; auto using instantiate_locals__updateAddAL).
+Case "sInsertValue". simpl_nd_llvmds. 
+  eapply instantiate_locals__getOperandValue in H; eauto.
+  destruct H as [gvs2 [J1 J2]].
+  eapply instantiate_locals__getOperandValue in H0; eauto.
+  destruct H0 as [gvs2' [J1' J2']].
+  eapply instantiate_locals__insertGenericValue in H1; eauto.
+  destruct H1 as [gvs2'' [J3 J4]].
+  exists (NDOS.mkState S' TD' Ps' 
+    ((NDOS.mkEC f1' b1' cs tmn1' (updateAddAL _ lc1' id0 gvs2'') als1')
+      ::ECs') gl' fs' M').
+  split; eauto.
+    repeat (split; auto using instantiate_locals__updateAddAL).
+Case "sMalloc". simpl_nd_llvmds. 
+  eapply instantiate_locals__getOperandValue in H0; eauto.
+  destruct H0 as [gns2 [J1 J2]].
+  exists (NDOS.mkState S' TD' Ps' 
+    ((NDOS.mkEC f1' b1' cs tmn1' 
+      (updateAddAL _ lc1' id0 (NDGVs.gv2gvs (blk2GV TD' mb) (typ_pointer t))) 
+    als1')::ECs') gl' fs' Mem').
+  split; eauto using instantiate_gvs__incl.
+    repeat (split; auto using instantiate_locals__updateAddAL, 
+                              instantiate_gvs__gv2gvs).
+Case "sFree". simpl_nd_llvmds. 
+  eapply instantiate_locals__getOperandValue in H; eauto.
+  destruct H as [gvs [J1 J2]].
+  exists (NDOS.mkState S' TD' Ps' 
+    ((NDOS.mkEC f1' b1' cs tmn1' lc1'
+    als1')::ECs') gl' fs' Mem').
+  split; eauto using instantiate_gvs__incl.
+    repeat (split; auto).
+Case "sAlloca". simpl_nd_llvmds. 
+  eapply instantiate_locals__getOperandValue in H0; eauto.
+  destruct H0 as [gns2 [J1 J2]].
+  exists (NDOS.mkState S' TD' Ps' 
+    ((NDOS.mkEC f1' b1' cs tmn1' 
+      (updateAddAL _ lc1' id0 (NDGVs.gv2gvs  (blk2GV TD' mb) (typ_pointer t))) 
+    (mb::als1'))::ECs') gl' fs' Mem').
+  split; eauto using instantiate_gvs__incl.
+    repeat (split; auto using instantiate_locals__updateAddAL, 
+                              instantiate_gvs__gv2gvs).
+Case "sLoad". simpl_nd_llvmds.
+  eapply instantiate_locals__getOperandValue in H; eauto.
+  destruct H as [gvs2 [J1 J2]].
+  exists (NDOS.mkState S' TD' Ps' 
+    ((NDOS.mkEC f1' b1' cs tmn1' (updateAddAL _ lc1' id0 (NDGVs.gv2gvs gv t))
+    als1')::ECs') gl' fs' M').
+  split; eauto using instantiate_gvs__incl.
+    repeat (split; auto using instantiate_locals__updateAddAL, 
+                              instantiate_gvs__gv2gvs).
+Case "sStore". simpl_nd_llvmds.
+  eapply instantiate_locals__getOperandValue in H; eauto.
+  destruct H as [gvs2 [J1 J2]].
+  eapply instantiate_locals__getOperandValue in H0; eauto.
+  destruct H0 as [mps2' [J3 J4]].
+  exists (NDOS.mkState S' TD' Ps' 
+    ((NDOS.mkEC f1' b1' cs tmn1' lc1' als1')::ECs') gl' fs' Mem').
+  split; eauto using instantiate_gvs__incl.
+    repeat (split; auto).
+Case "sGEP". simpl_nd_llvmds. 
+  eapply instantiate_locals__getOperandValue in H; eauto.
+  destruct H as [mps [J1 J2]].
+  eapply instantiate_locals__values2GVs in H0; eauto.
+  destruct H0 as [vidxss2 [J3 J4]].
+  eapply instantiate_locals__GEP in H1; eauto.
+  destruct H1 as [vidxs2 [mps2' [J5 [J6 J7]]]].
+  exists (NDOS.mkState S' TD' Ps' 
+    ((NDOS.mkEC f1' b1' cs tmn1' (updateAddAL _ lc1' id0 mps2') als1')
+      ::ECs') gl' fs' M').
+  split; eauto using instantiate_gvs__incl.
+    repeat (split; auto using instantiate_locals__updateAddAL).
+Case "sTrunc". simpl_nd_llvmds.
+  eapply instantiate_locals__TRUNC in H; eauto.
+  destruct H as [gvs2' [J1 J2]].
+  exists (NDOS.mkState S' TD' Ps' 
+    ((NDOS.mkEC f1' b1' cs tmn1' (updateAddAL _ lc1' id0 gvs2') als1')
+      ::ECs') gl' fs' M').
+  split; eauto using instantiate_gvs__incl.
+    repeat (split; auto using instantiate_locals__updateAddAL).
+Case "sExt". simpl_nd_llvmds. 
+  eapply instantiate_locals__EXT in H; eauto.
+  destruct H as [gvs2' [J1 J2]].
+  exists (NDOS.mkState S' TD' Ps' 
+    ((NDOS.mkEC f1' b1' cs tmn1' (updateAddAL _ lc1' id0 gvs2') als1')
+      ::ECs') gl' fs' M').
+  split; eauto using instantiate_gvs__incl.
+    repeat (split; auto using instantiate_locals__updateAddAL).
+Case "sCast". simpl_nd_llvmds. 
+  eapply instantiate_locals__CAST in H; eauto.
+  destruct H as [gvs2' [J1 J2]].
+  exists (NDOS.mkState S' TD' Ps' 
+    ((NDOS.mkEC f1' b1' cs tmn1' (updateAddAL _ lc1' id0 gvs2') als1')
+      ::ECs') gl' fs' M').
+  split; eauto using instantiate_gvs__incl.
+    repeat (split; auto using instantiate_locals__updateAddAL).
+Case "sIcmp". simpl_nd_llvmds. 
+  eapply instantiate_locals__ICMP in H; eauto.
+  destruct H as [gvs3' [J1 J2]].
+  exists (NDOS.mkState S' TD' Ps' 
+    ((NDOS.mkEC f1' b1' cs tmn1' (updateAddAL _ lc1' id0 gvs3') als1')
+      ::ECs') gl' fs' M').
+  split; eauto using instantiate_gvs__incl.
+    repeat (split; auto using instantiate_locals__updateAddAL).
+Case "sFcmp". simpl_nd_llvmds. 
+  eapply instantiate_locals__FCMP in H; eauto.
+  destruct H as [gvs3' [J1 J2]]. 
+  exists (NDOS.mkState S' TD' Ps' 
+    ((NDOS.mkEC f1' b1' cs tmn1' (updateAddAL _ lc1' id0 gvs3') als1')
+      ::ECs') gl' fs' M').
+  split; eauto using instantiate_gvs__incl.
+    repeat (split; auto using instantiate_locals__updateAddAL).
+Case "sSelect". simpl_nd_llvmds. 
+  eapply instantiate_locals__getOperandValue in H; eauto.
+  destruct H as [gvs0' [J1 J2]].
+  eapply instantiate_locals__getOperandValue in H0; eauto.
+  destruct H0 as [gvs1' [J3 J4]].
+  eapply instantiate_locals__getOperandValue in H1; eauto.
+  destruct H1 as [gvs2' [J5 J6]].
+  exists (NDOS.mkState S' TD' Ps' 
+    ((NDOS.mkEC f1' b1' cs tmn1' (if isGVZero TD' c 
+                                     then updateAddAL _ lc1' id0 gvs2' 
+                                     else updateAddAL _ lc1' id0 gvs1') als1')
+      ::ECs') gl' fs' M').
+  split; eauto using instantiate_gvs__incl.
+    repeat (split; auto).
+      destruct (isGVZero TD' c); auto using instantiate_locals__updateAddAL.
+Case "sCall". simpl_nd_llvmds. 
+  eapply instantiate_locals__getOperandValue in H; eauto.
+  destruct H as [gvs2 [J11 J12]].
+  eapply instantiate_locals__params2GVs in H3; eauto.
+  destruct H3 as [gvss2 [H11 H12]].
+  eapply instantiate_locals__initLocals in H4; eauto.
+  destruct H4 as [lc2' [H21 H22]].
+  exists (NDOS.mkState S' TD' Ps' 
+    ((NDOS.mkEC (fdef_intro (fheader_intro fa rt fid la va) lb) 
+                       (block_intro l' ps' cs' tmn') cs' tmn' lc2'
+                       nil)::
+     (NDOS.mkEC f1' b1' (insn_call rid noret0 ca ft fv lp :: cs) tmn1' 
+      lc1' als1') ::ECs') gl' fs' M').
+  split; eauto using instantiate_gvs__incl.
+    repeat (split; auto).
+Case "sExCall". simpl_nd_llvmds. 
+  eapply instantiate_locals__getOperandValue in H; eauto.
+  destruct H as [gvs2 [J11 J12]].
+  eapply instantiate_locals__params2GVs in H2; eauto.
+  destruct H2 as [gvss2 [H11 H12]].
+  eapply instantiate_locals__exCallUpdateLocals in H5; eauto.
+  destruct H5 as [lc2' [H21 H22]].
+  exists (NDOS.mkState S' TD' Ps' 
+    ((NDOS.mkEC f1' b1' cs tmn1' lc2' als1') ::ECs') gl' fs' Mem').
+  split.
+    eapply NDOS.sExCall; eauto using instantiate_gvs__incl,
+                                    instantiate_list_gvs__incl.
+    repeat (split; auto).
+Qed.
+
+
+(*****************************)
+(*
+*** Local Variables: ***
+*** coq-prog-name: "coqtop" ***
+*** coq-prog-args: ("-emacs-U" "-I" "~/SVN/sol/vol/src/ssa/monads" "-I" "~/SVN/sol/vol/src/ssa/ott" "-I" "~/SVN/sol/vol/src/ssa/compcert" "-I" "~/SVN/sol/theory/metatheory_8.3") ***
+*** End: ***
+ *)
